fiat2/src/fiat2/Language.v
@@ -11,7 +11,8 @@ Inductive type : Type :=
 | TList (t : type)
 | TRecord (l : list (string * type))
 | TDict (kt vt : type)
-| TBag (t : type).
+| TBag (t : type)
+| TSet (t : type).
 
 Section TypeIH.
   Context (P : type -> Prop).
@@ -19,7 +20,8 @@ Section TypeIH.
       (f_option : forall t : type, P t -> P (TOption t)) (f_list : forall t : type, P t -> P (TList t))
       (f_record : forall l : list (string * type), Forall (fun p => P (snd p)) l -> P (TRecord l))
       (f_dict : forall tk tv : type, P tk -> P tv -> P (TDict tk tv))
-      (f_bag : forall t : type, P t -> P (TBag t)).
+      (f_bag : forall t : type, P t -> P (TBag t))
+      (f_set : forall t : type, P t -> P (TSet t)).
     Section __.
       Context (type_IH : forall t, P t).
       Fixpoint record_type_IH (l : list (string * type)) : Forall (fun p => P (snd p)) l :=
@@ -40,6 +42,7 @@ Section TypeIH.
       | TRecord l => f_record l (record_type_IH type_IH l)
       | TDict tk tv => f_dict tk tv (type_IH tk) (type_IH tv)
       | TBag t => f_bag t (type_IH t)
+      | TSet t => f_set t (type_IH t)
        end.
 End TypeIH.
 
@@ -60,6 +63,7 @@ Inductive atom : Type :=
 | ANone (t : option type)
 | AEmptyDict (t : option (type * type))
 | AEmptyBag (t : option type)
+| AEmptySet (t : option type)
 | AUnit.
 
 (* Unary operators *)
@@ -98,6 +102,7 @@ Inductive binop : Type :=
 | ORange
 | OWRange
 | OBagInsert
+| OSetInsert
 | OLookup
 | ODelete.
 
@@ -106,9 +111,11 @@ Inductive ternop : Set :=
 | OInsert.
 
 (* What an expr with a list type can be interpreted to *)
-Inductive collection_tag := LikeBag | LikeList.
+Inductive collection_tag := LikeSet | LikeBag | LikeList.
 
 Inductive aggr := AGSum | AGCount.
+
+Inductive aci_aggr := AGMin | AGMax.
 
 (* Expressions *)
 Inductive expr : Type :=
@@ -124,6 +131,7 @@ Inductive expr : Type :=
 | EFlatmap2 (e1 e2 : expr) (x1 x2 : string) (e3 : expr)
 | EFold (e1 e2 : expr) (v acc : string) (e3 : expr)
 | EACFold (ag : aggr) (e : expr) (* associative commutative operation over bag *)
+| EACIFold (ag : aci_aggr) (e : expr) (* associative commutative idempotent operation over set *)
 | ERecord (l : list (string * expr))
 | EAccess (r : expr) (s : string)
 | EOptMatch (e : expr) (e_none : expr) (x : string) (e_some : expr)
@@ -133,7 +141,9 @@ Inductive expr : Type :=
 | EFilter (tag: collection_tag) (l : expr) (x : string) (p : expr) (* Select a subset of rows from table *)
 | EJoin (tag: collection_tag) (l1 l2 : expr) (x y : string) (p r : expr) (* Join two tables *)
 | EProj (tag: collection_tag) (l : expr) (x : string) (r : expr) (* Generalized projection *)
-| EBagOf (l : expr).
+(* conversion to different collections *)
+| EBagOf (l : expr)
+| ESetOf (l : expr).
 
 Section ExprIH.
   Context (P : expr -> Prop).
@@ -146,6 +156,7 @@ Section ExprIH.
     (f_flatmap : forall tag e1 x e2, P e1 -> P e2 -> P (EFlatmap tag e1 x e2))
     (f_flatmap2 : forall e1 e2 x1 x2 e3, P e1 -> P e2 -> P e3 -> P (EFlatmap2 e1 e2 x1 x2 e3))
     (f_acfold : forall ag e, P e -> P (EACFold ag e))
+    (f_acifold : forall ag e, P e -> P (EACIFold ag e))
     (f_fold : forall e1 e2 x y e3, P e1 -> P e2 -> P e3 -> P (EFold e1 e2 x y e3))
     (f_record : forall l, Forall (fun p => P (snd p)) l -> P (ERecord l))
     (f_access : forall r s, P r -> P (EAccess r s))
@@ -155,7 +166,8 @@ Section ExprIH.
     (f_filter : forall tag l x p, P l -> P p -> P (EFilter tag l x p))
     (f_join : forall tag l1 l2 x y p r, P l1 -> P l2 -> P p -> P r -> P (EJoin tag l1 l2 x y p r))
     (f_proj : forall tag l x r, P l -> P r -> P (EProj tag l x r))
-    (f_bagof : forall l, P l -> P (EBagOf l)).
+    (f_bagof : forall l, P l -> P (EBagOf l))
+    (f_setof : forall l, P l -> P (ESetOf l)).
 
     Section __.
       Context (expr_IH : forall e, P e).
@@ -180,6 +192,7 @@ Section ExprIH.
       | EFlatmap2 e1 e2 x1 x2 e3 => f_flatmap2 e1 e2 x1 x2 e3 (expr_IH e1) (expr_IH e2) (expr_IH e3)
       | EFold e1 e2 x y e3 => f_fold e1 e2 x y e3 (expr_IH e1) (expr_IH e2) (expr_IH e3)
       | EACFold ag e => f_acfold ag e (expr_IH e)
+      | EACIFold ag e => f_acifold ag e (expr_IH e)
       | ERecord l => f_record l (record_expr_IH expr_IH l)
       | EAccess r s => f_access r s (expr_IH r)
       | EOptMatch e e_none x e_some => f_optmatch e e_none x e_some (expr_IH e) (expr_IH e_none) (expr_IH e_some)
@@ -189,6 +202,7 @@ Section ExprIH.
       | EJoin tag l1 l2 x y p r => f_join tag l1 l2 x y p r (expr_IH l1) (expr_IH l2) (expr_IH p) (expr_IH r)
       | EProj tag l x r => f_proj tag l x r (expr_IH l) (expr_IH r)
       | EBagOf l => f_bagof l (expr_IH l)
+      | ESetOf l => f_setof l (expr_IH l)
       end.
 End ExprIH.
 
